{
 "cells": [
  {
   "cell_type": "markdown",
   "id": "2f4f0c13",
   "metadata": {},
   "source": [
    "$$ \\text{Gaussian}(\\mathbf{x}) = p(\\mathbf{x} | \\mathbf{\\mu}, \\mathbf{\\Sigma}) =\n",
    "\\frac{1}{\\sqrt{(2\\pi)^k |\\mathbf{\\Sigma}|}} \\exp{ \\bigg\\{-\\frac{1}{2}(\\mathbf{x} - \\mathbf{\\mu})^T \n",
    "\\mathbf{\\Sigma}^{-1} (\\mathbf{x} - \\mathbf{\\mu}) \n",
    "\\bigg\\} }\n",
    "$$\n",
    "\n",
    "<br>\n",
    "\n",
    "$$ \\{ \\mathbf{x}_i \\}_{i=1}^N $$\n"
   ]
  },
  {
   "cell_type": "markdown",
   "id": "a07042b2",
   "metadata": {},
   "source": [
    "$$ \\log \\mathcal{L}(\\mathbf{\\mu}, \\mathbf{\\Sigma}) = \\mathcal{l}(\\mathbf{\\mu}, \\mathbf{\\Sigma}) =\n",
    "\\log \\prod_{i=1}^{N} p(\\mathbf{x}_i | \\mathbf{\\mu}, \\mathbf{\\Sigma}) $$\n",
    "\n",
    "\n",
    "$$ = N\\log \\frac{1}{\\sqrt{(2\\pi)^k |\\mathbf{\\Sigma}|}} - \\frac{1}{2} \\sum_{i=1}^N (\\mathbf{x}_i - \\mathbf{\\mu})^T  \\mathbf{\\Sigma}^{-1} (\\mathbf{x}_i - \\mathbf{\\mu})  $$\n",
    "\n",
    "$$ = -\\frac{N}{2} \\log{(2\\pi)^k |\\mathbf{\\Sigma}|}  - \\frac{1}{2} \\sum_{i=1}^N (\\mathbf{x}_i - \\mathbf{\\mu})^T  \\mathbf{\\Sigma}^{-1} (\\mathbf{x}_i - \\mathbf{\\mu})  $$\n",
    "\n",
    "$$ = -\\frac{N}{2} \\log{(2\\pi)^k} -\\frac{N}{2}\\log{|\\mathbf{\\Sigma}|}  - \\frac{1}{2} \\sum_{i=1}^N (\\mathbf{x}_i - \\mathbf{\\mu})^T  \\mathbf{\\Sigma}^{-1} (\\mathbf{x}_i - \\mathbf{\\mu})  $$"
   ]
  },
  {
   "cell_type": "markdown",
   "id": "a47bc11e",
   "metadata": {},
   "source": [
    "\n",
    "$$ \\frac{\\partial \\mathcal{l}}{\\partial \\mathcal{\\mu}} = 0 $$\n",
    "\n",
    "\n",
    "$$ \\sum_{i=1}^N \\frac{\\partial}{\\partial \\mu} (\\mathbf{x}_i - \\mathbf{\\mu})^T  \\mathbf{\\Sigma}^{-1} (\\mathbf{x}_i - \\mathbf{\\mu}) = 0 $$\n",
    "\n",
    "<br>\n",
    "\n",
    "$$ \\mathbf{x}^T \\mathbf{B} \\mathbf{x} = 2\\mathbf{B} \\mathbf{x} $$\n",
    "\n",
    "<br>\n",
    "\n",
    "$$ 2 \\sum_{i=1}^N \\mathbf{\\Sigma}^{-1} (\\mathbf{x}_i - \\mathbf{\\mu}) = 0 $$\n",
    "\n",
    "$$ \\sum_{i=1}^N \\mathbf{\\Sigma}^{-1} \\mathbf{x}_i - \\sum_{i=1}^N \\mathbf{\\Sigma}^{-1} \\mathbf{\\mu} = 0 $$\n",
    "\n",
    "<br>\n",
    "\n",
    "$$ \\Sigma^{-1} \\ \\text{positive-definite} $$\n",
    "\n",
    "<br>\n",
    "\n",
    "$$ \\sum_{i=1}^N \\mathbf{x}_i =  \\sum_{i=1}^N \\mathbf{\\mu} $$\n",
    "\n",
    "\n",
    "\n",
    "$$ \\sum_{i=1}^N \\mathbf{x}_i =  N\\mathbf{\\mu} $$\n",
    "\n",
    "$$ \\mathbf{\\mu}  =  \\frac{1}{N} \\sum_{i=1}^N \\mathbf{x}_i = \\bar{\\mathbf{x}} $$"
   ]
  },
  {
   "cell_type": "markdown",
   "id": "699847e4",
   "metadata": {},
   "source": [
    "$$ \\mathcal{l}(\\mathbf{\\mu}, \\mathbf{\\Sigma}) = -\\frac{N}{2} \\log{(2\\pi)^k} -\\frac{N}{2}\\log{|\\mathbf{\\Sigma}|}  - \\frac{1}{2} \\sum_{i=1}^N (\\mathbf{x}_i - \\mathbf{\\mu})^T  \\mathbf{\\Sigma}^{-1} (\\mathbf{x}_i - \\mathbf{\\mu})  $$\n",
    "\n",
    "$$ |\\mathbf{\\Sigma}| = |\\mathbf{\\Sigma}^{-1}| $$\n",
    "\n",
    "$$ = -\\frac{N}{2} \\log{(2\\pi)^k} -\\frac{N}{2}\\log{|\\mathbf{\\Sigma}^{-1}|}  - \\frac{1}{2} \\sum_{i=1}^N (\\mathbf{x}_i - \\mathbf{\\mu})^T  \\mathbf{\\Sigma}^{-1} (\\mathbf{x}_i - \\mathbf{\\mu})  $$\n",
    "\n",
    "<br>\n",
    "\n",
    "$$ (\\mathbf{x}_i - \\mathbf{\\mu})^T  \\mathbf{\\Sigma}^{-1} (\\mathbf{x}_i - \\mathbf{\\mu}) \\in \\mathbb{R} $$\n",
    "$$ \\land$$\n",
    "$$ c = \\text{tr} (c) , \\ \\ \\ c \\in \\mathbb{R} $$\n",
    "\n",
    "$$ (\\mathbf{x}_i - \\mathbf{\\mu})^T  \\mathbf{\\Sigma}^{-1} (\\mathbf{x}_i - \\mathbf{\\mu}) = \\text{tr} \n",
    "\\big[  (\\mathbf{x}_i - \\mathbf{\\mu})^T  \\mathbf{\\Sigma}^{-1} (\\mathbf{x}_i - \\mathbf{\\mu})   \\big] $$\n",
    "\n",
    "<br>\n",
    "\n",
    "$$ = -\\frac{N}{2} \\log{(2\\pi)^k} -\\frac{N}{2}\\log{|\\mathbf{\\Sigma}^{-1}|}  - \\frac{1}{2} \\sum_{i=1}^N \\text{tr} \n",
    "\\big[  (\\mathbf{x}_i - \\mathbf{\\mu})^T  \\mathbf{\\Sigma}^{-1} (\\mathbf{x}_i - \\mathbf{\\mu})   \\big]  $$\n",
    "\n",
    "<br>\n",
    "\n",
    "$$ \\text{cyclic property} \\ \\ \\ \\ \\ \\text{tr}[ABC] = \\text{tr}[BCA] = \\text{tr}[CAB] $$\n",
    "\n",
    "<br>\n",
    "\n",
    "$$ = -\\frac{N}{2} \\log{(2\\pi)^k} -\\frac{N}{2}\\log{|\\mathbf{\\Sigma}^{-1}|}  - \\frac{1}{2} \\sum_{i=1}^N \\text{tr} \n",
    "\\big[ (\\mathbf{x}_i - \\mathbf{\\mu})  (\\mathbf{x}_i - \\mathbf{\\mu})^T  \\mathbf{\\Sigma}^{-1}   \\big]  $$"
   ]
  },
  {
   "cell_type": "markdown",
   "id": "c92bd8a9",
   "metadata": {},
   "source": [
    "$$ \\frac{\\partial\\mathcal{l}}{\\partial \\mathbf{\\Sigma}^{-1}} = 0 $$\n",
    "\n",
    "\n",
    "$$ \\frac{N}{2}\\mathbf{\\Sigma} - \\frac{1}{2} \\sum_{i=1}^N \\text(\\mathbf{x}_i - \\mathbf{\\mu})  (\\mathbf{x}_i - \\mathbf{\\mu})^T  = 0 $$\n",
    "\n",
    "$$ \\mathbf{\\Sigma} \n",
    "=  \\frac{1}{N} \\sum_{i=1}^N (\\mathbf{x}_i - \\mathbf{\\mu})  (\\mathbf{x}_i - \\mathbf{\\mu})^T $$"
   ]
  }
 ],
 "metadata": {
  "language_info": {
   "name": "python"
  }
 },
 "nbformat": 4,
 "nbformat_minor": 5
}
