{
 "cells": [
  {
   "cell_type": "markdown",
   "id": "33d221e5",
   "metadata": {},
   "source": [
    "\n",
    "Model\n",
    "\n",
    "$$ \\hat{Y} = \\phi(X; \\Theta) = \\Theta^T X + E $$\n",
    "\n",
    "\n",
    "Loss function\n",
    "$$ Q(\\Theta) = \\frac{1}{N} \\sum_{i=1}^N e_i^2 $$\n",
    "\n",
    "<br>\n",
    "\n",
    "$$ e_i = y_i - \\hat{y}_i  \\ \\ \\ \\ \\text{for} \\ \\ i = 1, \\dots, N $$\n",
    "\n",
    "\n",
    "\n",
    "$$ E = \n",
    "\\begin{bmatrix}\n",
    "e_1 & \\dots & e_N\n",
    "\\end{bmatrix} =\n",
    "\\begin{bmatrix}\n",
    "y_1 - \\hat{y}_1 & \\dots & y_N - \\hat{y}_N   \n",
    "\\end{bmatrix}\n",
    "$$\n",
    "\n",
    "<br>\n",
    "\n",
    "$$ (\\text{WLOG}) \\ \\ \\frac{1}{N} \\sum_{i=1}^N e_i^2 = \\sum_{i=1}^N e_i^2 $$\n",
    "\n",
    "$$\n",
    "\\sum_{i=1}^N e_i^2 = EE^T = (Y - \\hat{Y})(Y - \\hat{Y})^T = (Y - \\Theta^T X)(Y - \\Theta^T X)^T = \n",
    "$$\n",
    "\n",
    "$$\n",
    "= (Y - \\Theta^T X)(Y^T - X^T\\Theta) = YY^T - YX^T\\Theta - \\Theta^T XY^T + \\Theta X X^T \\Theta\n",
    "$$\n",
    "\n",
    "<br>\n",
    "\n",
    "$$ \n",
    "\\frac{\\partial Q}{\\partial \\Theta} = 0\n",
    "$$\n",
    "\n",
    "$$ \n",
    "\\frac{\\partial}{\\partial \\Theta}(YY^T - YX^T\\Theta - \\Theta^T XY^T + \\Theta X X^T \\Theta) = 0\n",
    "$$\n",
    "\n",
    "$$\n",
    "-XY^T - XY^T + 2XX^T \\Theta = 0\n",
    "$$\n",
    "\n",
    "\n",
    "$$\n",
    "XX^T \\Theta = XY^T\n",
    "$$\n",
    "\n",
    "$$\n",
    "\\Theta = (XX^T)^{-1}XY^T\n",
    "$$\n"
   ]
  }
 ],
 "metadata": {
  "language_info": {
   "name": "python"
  }
 },
 "nbformat": 4,
 "nbformat_minor": 5
}
